% Author: Aaron James Reynolds
% Date: January 14th, 2020

\documentclass[]{article}
\usepackage{geometry}
\usepackage{graphicx}
\geometry{textwidth=500pt}

\begin{document}
		\section*{\textbf{Prompt jump}} Start: PRKE. Assume: $\frac{\partial C(0)}{\partial t}=0$ and a single precursor group.\\\\
		Start with the delayed neutron precursor concentration equation at $t=0$.
		\[
		\frac{\partial}{\partial t}C(0) =\frac{\beta}{\Lambda}n(0)-\lambda C(0) 
		\]
		Assume $\frac{\partial C(0)}{\partial t}=0$
		\[
		0 =\frac{\beta}{\Lambda}n(0)-\lambda C(0) 
		\]
		\[
		C(0) =\frac{\beta}{\lambda\Lambda}n(0)
		\]
		Consider the neutron concentration equation and insert $C(0) =\frac{\beta}{\lambda\Lambda}n(0)$
		\[
		\frac{\partial}{\partial t}n(t)= \frac{\rho-\beta}{\Lambda}n(t)+\lambda C(0)
		\]
		\[
		\frac{\partial}{\partial t}n(t)- \frac{\rho-\beta}{\Lambda}n(t)=\frac{\beta}{\Lambda}n(0)
		\]
		Multiply by an integrating factor $e^{-\alpha t}$ where $\alpha = \frac{\rho-\beta}{\Lambda}$
		\[
		\frac{\partial n(t)}{\partial t}e^{-\alpha t}-\alpha n(t)e^{-\alpha t}=\frac{\beta}{\Lambda}n(0)e^{-\alpha t}
		\]
		\[
		\frac{\partial}{\partial t}n(t)e^{-\alpha t}=\frac{\beta}{\Lambda}n(0)e^{-\alpha t}
		\]
		Integrate with respect to $t$ from 0 to $t$.
		\[
		\int_{0}^{t}\frac{\partial}{\partial t}n(t)e^{-\alpha t}=\int_{0}^{t}\frac{\beta}{\Lambda}n(0)e^{-\alpha t}
		\]
		\[
		n(t)e^{-\alpha t}-n(0)=-\frac{\beta}{\alpha\Lambda}n(0)e^{-\alpha t} + \frac{\beta}{\alpha\Lambda}n(0)
		\]
		Divide by $n(0)$ and $e^{-\alpha t}$
		\[
		\frac{n(t)}{n(0)}e^{-\alpha t}=\frac{\beta}{\alpha\Lambda}(1-e^{-\alpha t}) +1
		\]
		\[
		\frac{n(t)}{n(0)}=\frac{\beta}{\alpha\Lambda}(e^{\alpha t}-1) +e^{\alpha t}
		\]
		\[
		\frac{n(t)}{n(0)}=-\frac{\beta}{\alpha\Lambda}+e^{\alpha t}(1+\frac{\beta}{\alpha\Lambda})
		\]
		Recall $\alpha = \frac{\rho-\beta}{\Lambda}$
		\[
		\frac{n(t)}{n(0)}=-\frac{\beta}{\Lambda}\frac{\Lambda}{\rho-\beta}+e^{\alpha t}(1+\frac{\beta}{\Lambda}\frac{\Lambda}{\rho-\beta})
		\]
		\[
		\frac{n(t)}{n(0)}=\frac{\beta}{\beta-\rho}+e^{\alpha t}(1-\frac{\beta}{\beta-\rho})
		\]
		Assume $\beta>>\rho$
		\[
		\frac{n(t)}{n(0)}=\frac{\beta}{\beta-\rho} = \frac{1}{1-\$}
		\]
		Above is the in-hour equation. If the system is not initially critical, the following equation applies.
		\[
		\frac{n_2}{n_1}=\frac{\beta-\rho_1}{\beta-\rho_2} = \frac{1-\$_1}{1-\$_2}
		\]
			
\end{document}